src/ModAdequacy.v
@@ -17,15 +17,50 @@ Set Implicit Arguments.
 
 
 
+Section AUX.
+
+  Definition alist_proj1 {K} {V} (a: alist K V): list K :=
+    List.map fst a.
+
+
+  Variable E1: Type -> Type.
+  Variable E2: Type -> Type.
+
+  Variable _ident_src: ID.
+  Variable _ident_tgt: ID.
+
+  Definition wf_ths {R}
+             (ths_src: @threads _ident_src E1 R)
+             (ths_tgt: @threads _ident_tgt E2 R) :=
+    (alist_proj1 ths_src) = (alist_proj1 ths_tgt).
+
+  Lemma ths_find_none_tid_add
+        R (ths: @threads _ident_src E1 R) tid
+        (NONE: threads_find tid ths = None)
+    :
+    tid_list_add (alist_proj1 ths) tid (tid :: (alist_proj1 ths)).
+  Proof.
+    revert_until ths. induction ths; i; ss.
+    { econs; ss. }
+    des_ifs. ss. destruct (tid_dec tid n) eqn:TID.
+    { clarify. eapply RelDec.neg_rel_dec_correct in Heq. ss. }
+    eapply IHths in NONE. inv NONE. econs; ss.
+    eapply List.not_in_cons. split; auto.
+  Qed.
+
+End AUX.
+
+
+
 Section ADEQ.
 
   Variable state_src: Type.
   Variable state_tgt: Type.
 
   Variable _ident_src: ID.
-  Definition ident_src := id_sum tids _ident_src.
+  Definition ident_src := sum_tids _ident_src.
   Variable _ident_tgt: ID.
-  Definition ident_tgt := id_sum tids _ident_tgt.
+  Definition ident_tgt := sum_tids _ident_tgt.
 
   Variable wf_src: WF.
   Variable wf_tgt: WF.
@@ -36,27 +71,30 @@ Section ADEQ.
   Variable world: Type.
   Variable world_le: world -> world -> Prop.
 
-  Variable I: (@shared state_src state_tgt ident_src ident_tgt wf_src wf_tgt world) -> Prop.
+  Variable I: (@shared state_src state_tgt _ident_src _ident_tgt wf_src wf_tgt world) -> Prop.
 
+  (*invariant for tid_list & threads: tid_list_add threads.proj1 tid tid_list*)
   Theorem local_adequacy
           R
+          (LSIM: forall (src0: itree srcE R) (tgt0: itree tgtE R),
+              local_sim world_le I src0 tgt0)
           (ths_src: @threads _ident_src (sE state_src) R)
           (ths_tgt: @threads _ident_tgt (sE state_tgt) R)
-          (LSIM: forall tid0 (src0: itree srcE R) (tgt0: itree tgtE R)
-                   (LSRC: Some src0 = threads_find tid0 ths_src)
-                   (LTGT: Some tgt0 = threads_find tid0 ths_tgt),
-              local_sim world_le I src0 tgt0)
           tid src tgt (st_src: state_src) (st_tgt: state_tgt)
-          (SRC: Some src = threads_find tid ths_src)
-          (TGT: Some tgt = threads_find tid ths_tgt)
-          (INV: forall im_tgt th_tgt, exists im_src th_src o w,
-              I ([], im_src, im_tgt, th_src, th_tgt, o, st_src, st_tgt, w))
+          (WFTHS: wf_ths ths_src ths_tgt)
+          (THSRC: threads_find tid ths_src = None)
+          (THTGT: threads_find tid ths_tgt = None)
+          (INV: forall im_tgt, exists im_src o w,
+              I (alist_proj1 ths_src, im_src, im_tgt, st_src, st_tgt, o, w))
     :
     gsim wf_src wf_tgt (@eq R) false false
          (interp_all st_src ths_src tid src)
          (interp_all st_tgt ths_tgt tid tgt).
   Proof.
-    ii.
+    ii. specialize (INV mt). des. rename im_src into ms. exists ms.
+    pose proof (ths_find_none_tid_add ths_src tid THSRC) as TADD. 
+    unfold local_sim in LSIM. specialize (LSIM src tgt _ _ _ _ _ _ _ INV tid _ TADD).
+
 
   Abort.
 
