src/ModSimPico.v
@@ -15,8 +15,10 @@ Section PRIMIVIESIM.
   Variable state_src: Type.
   Variable state_tgt: Type.
 
-  Variable ident_src: ID.
-  Variable ident_tgt: ID.
+  Variable _ident_src: ID.
+  Definition ident_src := sum_tids _ident_src.
+  Variable _ident_tgt: ID.
+  Definition ident_tgt := sum_tids _ident_tgt.
 
   Variable wf_src: WF.
   Variable wf_tgt: WF.
@@ -32,22 +34,22 @@ Section PRIMIVIESIM.
     (tid_list *
        (@imap ident_src wf_src) *
        (@imap ident_tgt wf_tgt) *
-       (@imap tids wf_src) *
-       (@imap tids wf_tgt) *
-       wf_src.(T) *
+       (* (@imap tids wf_src) * *)
+       (* (@imap tids wf_tgt) * *)
        state_src *
        state_tgt *
+       wf_src.(T) *
        world)%type.
 
   Let shared_rel: Type := shared -> Prop.
 
   Definition shared_rel_wf (r: shared_rel): Prop :=
-    forall ths im_src im_tgt th_src0 th_tgt0 o st_src st_tgt w0
-      (INV: r (ths, im_src, im_tgt, th_src0, th_tgt0, o, st_src, st_tgt, w0))
-      th_tgt1 (TGT: fair_update th_tgt0 th_tgt1 (fun _ => Flag.fail)),
-    exists th_src1 w1,
-      (<<SRC: fair_update th_src0 th_src1 (fun _ => Flag.fail)>>) /\
-        (<<INV: r (ths, im_src, im_tgt, th_src1, th_tgt1, o, st_src, st_tgt, w1)>>) /\
+    forall ths im_src0 im_tgt0 st_src st_tgt o w0
+      (INV: r (ths, im_src0, im_tgt0, st_src, st_tgt, o, w0))
+      im_tgt1 (TGT: fair_update im_tgt0 im_tgt1 (sum_fmap_l (fun _ => Flag.fail))),
+    exists im_src1 w1,
+      (<<SRC: fair_update im_src0 im_src1 (sum_fmap_l (fun _ => Flag.fail))>>) /\
+        (<<INV: r (ths, im_src1, im_tgt1, st_src, st_tgt, o, w1)>>) /\
         (<<WORLD: world_le w0 w1>>).
 
   Variable I: shared_rel.
@@ -62,148 +64,148 @@ Section PRIMIVIESIM.
     bool -> bool -> itree srcE R_src -> itree tgtE R_tgt -> shared_rel :=
   | lsim_ret
       f_src f_tgt
-      ths im_src im_tgt th_src th_tgt o st_src st_tgt w
+      ths im_src im_tgt st_src st_tgt o w
       r_src r_tgt
-      (LSIM: RR r_src r_tgt (ths, im_src, im_tgt, th_src, th_tgt, o, st_src, st_tgt, w))
+      (LSIM: RR r_src r_tgt (ths, im_src, im_tgt, st_src, st_tgt, o, w))
     :
-    __lsim tid lsim _lsim RR f_src f_tgt (Ret r_src) (Ret r_tgt) (ths, im_src, im_tgt, th_src, th_tgt, o, st_src, st_tgt, w)
+    __lsim tid lsim _lsim RR f_src f_tgt (Ret r_src) (Ret r_tgt) (ths, im_src, im_tgt, st_src, st_tgt, o, w)
 
   | lsim_tauL
       f_src f_tgt
-      ths im_src im_tgt th_src th_tgt o st_src st_tgt w
+      ths im_src im_tgt st_src st_tgt o w
       itr_src itr_tgt
-      (LSIM: _lsim _ _ RR true f_tgt itr_src itr_tgt (ths, im_src, im_tgt, th_src, th_tgt, o, st_src, st_tgt, w))
+      (LSIM: _lsim _ _ RR true f_tgt itr_src itr_tgt (ths, im_src, im_tgt, st_src, st_tgt, o, w))
     :
-    __lsim tid lsim _lsim RR f_src f_tgt (Tau itr_src) itr_tgt (ths, im_src, im_tgt, th_src, th_tgt, o, st_src, st_tgt, w)
+    __lsim tid lsim _lsim RR f_src f_tgt (Tau itr_src) itr_tgt (ths, im_src, im_tgt, st_src, st_tgt, o, w)
   | lsim_chooseL
       f_src f_tgt
-      ths im_src im_tgt th_src th_tgt o st_src st_tgt w
+      ths im_src im_tgt st_src st_tgt o w
       X ktr_src itr_tgt
-      (LSIM: exists x, _lsim _ _ RR true f_tgt (ktr_src x) itr_tgt (ths, im_src, im_tgt, th_src, th_tgt, o, st_src, st_tgt, w))
+      (LSIM: exists x, _lsim _ _ RR true f_tgt (ktr_src x) itr_tgt (ths, im_src, im_tgt, st_src, st_tgt, o, w))
     :
-    __lsim tid lsim _lsim RR f_src f_tgt (trigger (Choose X) >>= ktr_src) itr_tgt (ths, im_src, im_tgt, th_src, th_tgt, o, st_src, st_tgt, w)
+    __lsim tid lsim _lsim RR f_src f_tgt (trigger (Choose X) >>= ktr_src) itr_tgt (ths, im_src, im_tgt, st_src, st_tgt, o, w)
   | lsim_putL
       f_src f_tgt
-      ths im_src im_tgt th_src th_tgt o st_src st_tgt w
+      ths im_src im_tgt st_src st_tgt o w
       st ktr_src itr_tgt
-      (LSIM: _lsim _ _ RR true f_tgt (ktr_src tt) itr_tgt (ths, im_src, im_tgt, th_src, th_tgt, o, st, st_tgt, w))
+      (LSIM: _lsim _ _ RR true f_tgt (ktr_src tt) itr_tgt (ths, im_src, im_tgt, st, st_tgt, o, w))
     :
-    __lsim tid lsim _lsim RR f_src f_tgt (trigger (Put st) >>= ktr_src) itr_tgt (ths, im_src, im_tgt, th_src, th_tgt, o, st_src, st_tgt, w)
+    __lsim tid lsim _lsim RR f_src f_tgt (trigger (Put st) >>= ktr_src) itr_tgt (ths, im_src, im_tgt, st_src, st_tgt, o, w)
   | lsim_getL
       f_src f_tgt
-      ths im_src im_tgt th_src th_tgt o st_src st_tgt w
+      ths im_src im_tgt st_src st_tgt o w
       ktr_src itr_tgt
-      (LSIM: _lsim _ _ RR true f_tgt (ktr_src st_src) itr_tgt (ths, im_src, im_tgt, th_src, th_tgt, o, st_src, st_tgt, w))
+      (LSIM: _lsim _ _ RR true f_tgt (ktr_src st_src) itr_tgt (ths, im_src, im_tgt, st_src, st_tgt, o, w))
     :
-    __lsim tid lsim _lsim RR f_src f_tgt (trigger (@Get _) >>= ktr_src) itr_tgt (ths, im_src, im_tgt, th_src, th_tgt, o, st_src, st_tgt, w)
+    __lsim tid lsim _lsim RR f_src f_tgt (trigger (@Get _) >>= ktr_src) itr_tgt (ths, im_src, im_tgt, st_src, st_tgt, o, w)
   | lsim_tidL
       f_src f_tgt
-      ths im_src im_tgt th_src th_tgt o st_src st_tgt w
+      ths im_src im_tgt st_src st_tgt o w
       ktr_src itr_tgt
-      (LSIM: _lsim _ _ RR true f_tgt (ktr_src tid) itr_tgt (ths, im_src, im_tgt, th_src, th_tgt, o, st_src, st_tgt, w))
+      (LSIM: _lsim _ _ RR true f_tgt (ktr_src tid) itr_tgt (ths, im_src, im_tgt, st_src, st_tgt, o, w))
     :
-    __lsim tid lsim _lsim RR f_src f_tgt (trigger (GetTid) >>= ktr_src) itr_tgt (ths, im_src, im_tgt, th_src, th_tgt, o, st_src, st_tgt, w)
+    __lsim tid lsim _lsim RR f_src f_tgt (trigger (GetTid) >>= ktr_src) itr_tgt (ths, im_src, im_tgt, st_src, st_tgt, o, w)
   | lsim_UB
       f_src f_tgt
-      ths im_src im_tgt th_src th_tgt o st_src st_tgt w
+      ths im_src im_tgt st_src st_tgt o w
       ktr_src itr_tgt
     :
-    __lsim tid lsim _lsim RR f_src f_tgt (trigger (Undefined) >>= ktr_src) itr_tgt (ths, im_src, im_tgt, th_src, th_tgt, o, st_src, st_tgt, w)
+    __lsim tid lsim _lsim RR f_src f_tgt (trigger (Undefined) >>= ktr_src) itr_tgt (ths, im_src, im_tgt, st_src, st_tgt, o, w)
   | lsim_fairL
       f_src f_tgt
-      ths im_src0 im_tgt th_src th_tgt o st_src st_tgt w
+      ths im_src0 im_tgt st_src st_tgt o w
       f ktr_src itr_tgt
       (LSIM: exists im_src1,
           (<<FAIR: fair_update im_src0 im_src1 f>>) /\
-            (<<LSIM: _lsim _ _ RR true f_tgt (ktr_src tt) itr_tgt (ths, im_src1, im_tgt, th_src, th_tgt, o, st_src, st_tgt, w)>>))
+            (<<LSIM: _lsim _ _ RR true f_tgt (ktr_src tt) itr_tgt (ths, im_src1, im_tgt, st_src, st_tgt, o, w)>>))
     :
-    __lsim tid lsim _lsim RR f_src f_tgt (trigger (Fair f) >>= ktr_src) itr_tgt (ths, im_src0, im_tgt, th_src, th_tgt, o, st_src, st_tgt, w)
+    __lsim tid lsim _lsim RR f_src f_tgt (trigger (Fair f) >>= ktr_src) itr_tgt (ths, im_src0, im_tgt, st_src, st_tgt, o, w)
 
   | lsim_tauR
       f_src f_tgt
-      ths im_src im_tgt th_src th_tgt o st_src st_tgt w
+      ths im_src im_tgt st_src st_tgt o w
       itr_src itr_tgt
-      (LSIM: _lsim _ _ RR f_src true itr_src itr_tgt (ths, im_src, im_tgt, th_src, th_tgt, o, st_src, st_tgt, w))
+      (LSIM: _lsim _ _ RR f_src true itr_src itr_tgt (ths, im_src, im_tgt, st_src, st_tgt, o, w))
     :
-    __lsim tid lsim _lsim RR f_src f_tgt itr_src (Tau itr_tgt) (ths, im_src, im_tgt, th_src, th_tgt, o, st_src, st_tgt, w)
+    __lsim tid lsim _lsim RR f_src f_tgt itr_src (Tau itr_tgt) (ths, im_src, im_tgt, st_src, st_tgt, o, w)
   | lsim_chooseR
       f_src f_tgt
-      ths im_src im_tgt th_src th_tgt o st_src st_tgt w
+      ths im_src im_tgt st_src st_tgt o w
       X itr_src ktr_tgt
-      (LSIM: forall x, _lsim _ _ RR f_src true itr_src (ktr_tgt x) (ths, im_src, im_tgt, th_src, th_tgt, o, st_src, st_tgt, w))
+      (LSIM: forall x, _lsim _ _ RR f_src true itr_src (ktr_tgt x) (ths, im_src, im_tgt, st_src, st_tgt, o, w))
     :
-    __lsim tid lsim _lsim RR f_src f_tgt itr_src (trigger (Choose X) >>= ktr_tgt) (ths, im_src, im_tgt, th_src, th_tgt, o, st_src, st_tgt, w)
+    __lsim tid lsim _lsim RR f_src f_tgt itr_src (trigger (Choose X) >>= ktr_tgt) (ths, im_src, im_tgt, st_src, st_tgt, o, w)
   | lsim_putR
       f_src f_tgt
-      ths im_src im_tgt th_src th_tgt o st_src st_tgt w
+      ths im_src im_tgt st_src st_tgt o w
       st itr_src ktr_tgt
-      (LSIM: _lsim _ _ RR f_src true itr_src (ktr_tgt tt) (ths, im_src, im_tgt, th_src, th_tgt, o, st_src, st, w))
+      (LSIM: _lsim _ _ RR f_src true itr_src (ktr_tgt tt) (ths, im_src, im_tgt, st_src, st, o, w))
     :
-    __lsim tid lsim _lsim RR f_src f_tgt itr_src (trigger (Put st) >>= ktr_tgt) (ths, im_src, im_tgt, th_src, th_tgt, o, st_src, st_tgt, w)
+    __lsim tid lsim _lsim RR f_src f_tgt itr_src (trigger (Put st) >>= ktr_tgt) (ths, im_src, im_tgt, st_src, st_tgt, o, w)
   | lsim_getR
       f_src f_tgt
-      ths im_src im_tgt th_src th_tgt o st_src st_tgt w
+      ths im_src im_tgt st_src st_tgt o w
       itr_src ktr_tgt
-      (LSIM: _lsim _ _ RR f_src true itr_src (ktr_tgt st_tgt) (ths, im_src, im_tgt, th_src, th_tgt, o, st_src, st_tgt, w))
+      (LSIM: _lsim _ _ RR f_src true itr_src (ktr_tgt st_tgt) (ths, im_src, im_tgt, st_src, st_tgt, o, w))
     :
-    __lsim tid lsim _lsim RR f_src f_tgt itr_src (trigger (@Get _) >>= ktr_tgt) (ths, im_src, im_tgt, th_src, th_tgt, o, st_src, st_tgt, w)
+    __lsim tid lsim _lsim RR f_src f_tgt itr_src (trigger (@Get _) >>= ktr_tgt) (ths, im_src, im_tgt, st_src, st_tgt, o, w)
   | lsim_tidR
       f_src f_tgt
-      ths im_src im_tgt th_src th_tgt o st_src st_tgt w
+      ths im_src im_tgt st_src st_tgt o w
       itr_src ktr_tgt
-      (LSIM: _lsim _ _ RR f_src true itr_src (ktr_tgt tid) (ths, im_src, im_tgt, th_src, th_tgt, o, st_src, st_tgt, w))
+      (LSIM: _lsim _ _ RR f_src true itr_src (ktr_tgt tid) (ths, im_src, im_tgt, st_src, st_tgt, o, w))
     :
-    __lsim tid lsim _lsim RR f_src f_tgt itr_src (trigger (GetTid) >>= ktr_tgt) (ths, im_src, im_tgt, th_src, th_tgt, o, st_src, st_tgt, w)
+    __lsim tid lsim _lsim RR f_src f_tgt itr_src (trigger (GetTid) >>= ktr_tgt) (ths, im_src, im_tgt, st_src, st_tgt, o, w)
   | lsim_fairR
       f_src f_tgt
-      ths im_src im_tgt0 th_src th_tgt o st_src st_tgt w
+      ths im_src im_tgt0 st_src st_tgt o w
       f itr_src ktr_tgt
       (LSIM: forall im_tgt1
                    (FAIR: fair_update im_tgt0 im_tgt1 f),
-          (<<LSIM: _lsim _ _ RR f_src true itr_src (ktr_tgt tt) (ths, im_src, im_tgt1, th_src, th_tgt, o, st_src, st_tgt, w)>>))
+          (<<LSIM: _lsim _ _ RR f_src true itr_src (ktr_tgt tt) (ths, im_src, im_tgt1, st_src, st_tgt, o, w)>>))
     :
-    __lsim tid lsim _lsim RR f_src f_tgt itr_src (trigger (Fair f) >>= ktr_tgt) (ths, im_src, im_tgt0, th_src, th_tgt, o, st_src, st_tgt, w)
+    __lsim tid lsim _lsim RR f_src f_tgt itr_src (trigger (Fair f) >>= ktr_tgt) (ths, im_src, im_tgt0, st_src, st_tgt, o, w)
 
   | lsim_observe
       f_src f_tgt
-      ths im_src im_tgt th_src th_tgt o st_src st_tgt w
+      ths im_src im_tgt st_src st_tgt o w
       fn args ktr_src ktr_tgt
       (LSIM: forall ret,
-          lsim _ _ RR true true (ktr_src ret) (ktr_tgt ret) (ths, im_src, im_tgt, th_src, th_tgt, o, st_src, st_tgt, w))
+          lsim _ _ RR true true (ktr_src ret) (ktr_tgt ret) (ths, im_src, im_tgt, st_src, st_tgt, o, w))
     :
-    __lsim tid lsim _lsim RR f_src f_tgt (trigger (Observe fn args) >>= ktr_src) (trigger (Observe fn args) >>= ktr_tgt) (ths, im_src, im_tgt, th_src, th_tgt, o, st_src, st_tgt, w)
+    __lsim tid lsim _lsim RR f_src f_tgt (trigger (Observe fn args) >>= ktr_src) (trigger (Observe fn args) >>= ktr_tgt) (ths, im_src, im_tgt, st_src, st_tgt, o, w)
 
   | lsim_sync
       f_src f_tgt
-      ths0 im_src0 im_tgt0 th_src0 th_tgt0 o st_src0 st_tgt0 w
+      ths0 im_src0 im_tgt0 st_src0 st_tgt0 o w
       o0 w0 ktr_src ktr_tgt
-      (INV: I (ths0, im_src0, im_tgt0, th_src0, th_tgt0, o0, st_src0, st_tgt0, w0))
+      (INV: I (ths0, im_src0, im_tgt0, st_src0, st_tgt0, o0, w0))
       (WORLD: world_le w w0)
       (STUTTER: wf_src.(lt) o0 o)
-      (LSIM: forall ths1 im_src1 im_tgt1 th_src1 th_tgt1 o1 st_src1 st_tgt1 w1
-                   (INV: I (ths1, im_src1, im_tgt1, th_src1, th_tgt1, o1, st_src1, st_tgt1, w1))
+      (LSIM: forall ths1 im_src1 im_tgt1 st_src1 st_tgt1 o1 w1
+                   (INV: I (ths1, im_src1, im_tgt1, st_src1, st_tgt1, o1, w1))
                    (WORLD: world_le w0 w1)
-                   th_tgt2
-                   (TGT: fair_update th_tgt1 th_tgt2 (thread_fmap tid)),
-          lsim _ _ RR true true (trigger (Yield) >>= ktr_src) (ktr_tgt tt) (ths1, im_src1, im_tgt1, th_src1, th_tgt2, o1, st_src1, st_tgt1, w1))
+                   im_tgt2
+                   (TGT: fair_update im_tgt1 im_tgt2 (sum_fmap_l (thread_fmap tid))),
+          lsim _ _ RR true true (trigger (Yield) >>= ktr_src) (ktr_tgt tt) (ths1, im_src1, im_tgt2, st_src1, st_tgt1, o1, w1))
     :
-    __lsim tid lsim _lsim RR f_src f_tgt (trigger (Yield) >>= ktr_src) (trigger (Yield) >>= ktr_tgt) (ths0, im_src0, im_tgt0, th_src0, th_tgt0, o, st_src0, st_tgt0, w)
+    __lsim tid lsim _lsim RR f_src f_tgt (trigger (Yield) >>= ktr_src) (trigger (Yield) >>= ktr_tgt) (ths0, im_src0, im_tgt0, st_src0, st_tgt0, o, w)
   | lsim_yieldL
       f_src f_tgt
-      ths im_src im_tgt th_src0 th_tgt o0 st_src st_tgt w
+      ths im_src0 im_tgt st_src st_tgt o0 w
       ktr_src itr_tgt
-      (LSIM: exists th_src1 o1,
-          (<<FAIR: fair_update th_src0 th_src1 (thread_fmap tid)>>) /\
-            (<<LSIM: _lsim _ _ RR true f_tgt (ktr_src tt) itr_tgt (ths, im_src, im_tgt, th_src1, th_tgt, o1, st_src, st_tgt, w)>>))
+      (LSIM: exists im_src1 o1,
+          (<<FAIR: fair_update im_src0 im_src1 (sum_fmap_l (thread_fmap tid))>>) /\
+            (<<LSIM: _lsim _ _ RR true f_tgt (ktr_src tt) itr_tgt (ths, im_src1, im_tgt, st_src, st_tgt, o1, w)>>))
     :
-    __lsim tid lsim _lsim RR f_src f_tgt (trigger (Yield) >>= ktr_src) itr_tgt (ths, im_src, im_tgt, th_src0, th_tgt, o0, st_src, st_tgt, w)
+    __lsim tid lsim _lsim RR f_src f_tgt (trigger (Yield) >>= ktr_src) itr_tgt (ths, im_src0, im_tgt, st_src, st_tgt, o0, w)
 
   | lsim_progress
-      ths im_src im_tgt th_src th_tgt o st_src st_tgt w
+      ths im_src im_tgt st_src st_tgt o w
       itr_src itr_tgt
-      (LSIM: lsim _ _ RR false false itr_src itr_tgt (ths, im_src, im_tgt, th_src, th_tgt, o, st_src, st_tgt, w))
+      (LSIM: lsim _ _ RR false false itr_src itr_tgt (ths, im_src, im_tgt, st_src, st_tgt, o, w))
     :
-    __lsim tid lsim _lsim RR true true itr_src itr_tgt (ths, im_src, im_tgt, th_src, th_tgt, o, st_src, st_tgt, w)
+    __lsim tid lsim _lsim RR true true itr_src itr_tgt (ths, im_src, im_tgt, st_src, st_tgt, o, w)
   .
 
   Definition lsim (tid: tids.(id)): forall R_src R_tgt (RR: R_src -> R_tgt -> shared_rel),
@@ -231,16 +233,16 @@ Section PRIMIVIESIM.
   Qed.
 
   Definition local_RR {R} tid :=
-    fun (r_src r_tgt: R) '(ths2, im_src1, im_tgt1, th_src1, th_tgt1, o1, st_src1, st_tgt1, w1) =>
+    fun (r_src r_tgt: R) '(ths2, im_src1, im_tgt1, st_src1, st_tgt1, o1, w1) =>
       exists ths3 w2,
         (<<THS: tid_list_remove ths2 tid ths3>>) /\
           (<<WORLD: world_le w1 w2>>) /\
-          (<<INV: I (ths3, im_src1, im_tgt1, th_src1, th_tgt1, o1, st_src1, st_tgt1, w2)>>) /\
+          (<<INV: I (ths3, im_src1, im_tgt1, st_src1, st_tgt1, o1, w2)>>) /\
           (<<RET: r_src = r_tgt>>).
 
   Definition local_sim {R} src tgt :=
-    forall ths0 im_src0 im_tgt0 th_src0 th_tgt0 o0 st_src0 st_tgt0 w0
-      (INV: I (ths0, im_src0, im_tgt0, th_src0, th_tgt0, o0, st_src0, st_tgt0, w0))
+    forall ths0 im_src0 im_tgt0 st_src0 st_tgt0 o0 w0
+      (INV: I (ths0, im_src0, im_tgt0, st_src0, st_tgt0, o0, w0))
       tid ths1
       (THS: tid_list_add ths0 tid ths1),
       lsim
@@ -248,11 +250,12 @@ Section PRIMIVIESIM.
         (@local_RR R tid)
         false false
         src tgt
-        (ths1, im_src0, im_tgt0, th_src0, th_tgt0, o0, st_src0, st_tgt0, w0).
+        (ths1, im_src0, im_tgt0, st_src0, st_tgt0, o0, w0).
 
 End PRIMIVIESIM.
 #[export] Hint Constructors __lsim: core.
 #[export] Hint Unfold lsim: core.
+#[export] Hint Resolve __lsim_mon: paco.
 #[export] Hint Resolve _lsim_mon: paco.
 #[export] Hint Resolve lsim_mon: paco.
 
@@ -269,11 +272,10 @@ Module ModSim.
           wf: WF;
           world: Type;
           world_le: world -> world -> Prop;
-          I: (@shared md_src.(Mod.state) md_tgt.(Mod.state) md_src.(Mod.ident) md_tgt.(Mod.ident) wf nat_wf world) -> Prop;
+          I: (@shared md_src.(Mod.state) md_tgt.(Mod.state) md_src.(Mod._ident) md_tgt.(Mod._ident) wf nat_wf world) -> Prop;
 
-          init: forall im_tgt th_tgt,
-          exists im_src th_src o w,
-            I ([], im_src, im_tgt, th_src, th_tgt, o, md_src.(Mod.st_init), md_tgt.(Mod.st_init), w);
+          init: forall im_tgt, exists im_src o w,
+            I ([], im_src, im_tgt, md_src.(Mod.st_init), md_tgt.(Mod.st_init), o, w);
 
           funs: forall fn args, local_sim world_le I (md_src.(Mod.funs) fn args) (md_tgt.(Mod.funs) fn args);
         }.
